\documentclass[UTF8]{ctexart}
\usepackage{amsmath}
\usepackage{mathtools}
\usepackage{geometry}
\title{二次函数的有关计算}
\author{}
\geometry{a4paper,scale=0.75}
\begin{document}


\maketitle
\begin{flushleft}
已知:二次函数$y=ax^{2}+bx+c$过三点$(x_{1},y_{1}),(x_{2},y_{2}),(x_{3},y_{3})$,求该函数的解析式.\\
解:将点$(x_{1},y_{1}),(x_{2},y_{2}),(x_{3},y_{3})$代入解析式,得
\end{flushleft}
\[
\begin{cases}
y_{1}=ax_{1}^{2}+bx_{1}+c\quad (1)\\
y_{2}=ax_{2}^{2}+bx_{2}+c\quad (2)\\
y_{3}=ax_{3}^{2}+bx_{3}+c\quad (3)\\
\end{cases}
\]

$(1)-(2),(2)-(3)$,得\\
\[
\begin{cases}
y_{1}-y_{2}=a(x_{1}^{2}-x_{2}^{2})+b(x_{1}-x_{2})\quad (4)\\
y_{2}-y_{3}=a(x_{2}^{2}-x_{3}^{2})+b(x_{2}-x_{3})\quad (5)\\
\end{cases}
\]
$(4)\times (x_{2}-x_{3})-(5)\times (x_{1}-x_{2})$得
\[(y_{1}-y_{2})(x_{2}-x_{3})-(y_{2}-y_{3})(x_{1}-x_{2})\]
\[=a\times [(x_{1}^{2}-x_{2}^{2})(x_{2}-x_{3})-(x_{2}^{2}-x_{3}^{2})(x_{1}-x_{2})]\]
即
\[
\begin{aligned}
a&=\frac{(y_{1}-y_{2})(x_{2}-x_{3})-(y_{2}-y_{3})(x_{1}-x_{2})}{(x_{1}^{2}-x_{2}^{2})(x_{2}-x_{3})-(x_{2}^{2}-x_{3}^{2})(x_{1}-x_{2})}\\
& \\
&=-\frac{\sum\limits_{cyc}x_{1}(y_{2}-y_{3})}{\sum\limits_{cyc}x_{1}^{2}(y_{2}-y_{3})}\\
\end{aligned}
\]
 
$(4)\times (x_{2}^{2}-x_{3}^{2})-(5)\times (x_{1}^{2}-x_{2}^{2})$,得
\[(y_{1}-y_{2})(x_{2}^{2}-x_{3}^{2})-(y_{2}-y_{3})(x_{1}^{2}-x_{2}^{2})\]
\[=b \times [(x_{1}-x_{2})(x_{2}^{2}-x_{3}^{2})-(x_{2}-x_{3})(x_{1}^{2}-x_{2}^{2})]\]
即
\[
\begin{aligned}
b&=\frac{(y_{1}-y_{2})(x_{2}^{2}-x_{3}^{2})-(y_{2}-y_{3})(x_{1}^{2}-x_{2}^{2})}{(x_{1}-x_{2})(x_{2}^{2}-x_{3}^{2})-(x_{2}-x_{3})(x_{1}^{2}-x_{2}^{2})}\\
& \\
&=\frac{\sum\limits_{cyc}x_{1}^{2}(y_{2}-y_{3})}{\sum\limits_{cyc}x_{1}^{2}(x_{2}-x_{3})}\\
\end{aligned}
\]

$(1) \times x_{2}x_{3},(2) \times x_{3}x_{1},(3) \times x_{1}x_{2}$,得
\[
\begin{cases}
y_{1}x_{2}x_{3}=ax_{1}^{2}x_{2}x_{3}+bx_{1}x_{2}x_{3}+cx_{2}x_{3}\quad (6)\\
y_{2}x_{3}x_{1}=ax_{2}^{2}x_{3}x_{1}+bx_{2}x_{3}x_{1}+cx_{3}x_{1}\quad (7)\\
y_{3}x_{1}x_{2}=ax_{3}^{2}x_{1}x_{2}+bx_{3}x_{1}x_{2}+cx_{1}x_{2}\quad (8)\\
\end{cases}
\]
$(6)-(7),(7)-(8)$,得
\[
\begin{cases}
x_{3}(y_{1}x_{2}-y_{2}x_{1})=ax_{1}x_{2}x_{3}(x_{1}-x_{2})+cx_{3}(x_{2}-x_{1})\quad (9)\\
x_{1}(y_{2}x_{3}-y_{3}x_{2})=ax_{2}x_{3}x_{1}(x_{2}-x_{3})+cx_{1}(x_{3}-x_{2})\quad (10)\\
\end{cases}
\]
$(9)\times(x_{2}-x_{3})-(10)\times(x_{1}-x_{2})$,得
\[x_{3}(x_{2}-x_{3})(y_{1}x_{2}-y_{2}x_{1})-x_{1}(x_{1}-x_{2})(y_{2}x_{3}-y_{3}x_{2})\]
\[=c\times[x_{3}(x_{2}-x_{1})(x_{2}-x_{3})-x_{1}(x_{3}-x_{2})(x_{1}-x_{2})]\]
即
\[
\begin{aligned}
c&=\frac{x_{3}(x_{2}-x_{3})(y_{1}x_{2}-y_{2}x_{1})-x_{1}(x_{1}-x_{2})(y_{2}x_{3}-y_{3}x_{2})}{x_{3}(x_{2}-x_{1})(x_{2}-x_{3})-x_{1}(x_{3}-x_{2})(x_{1}-x_{2})}\\
& \\
&=\frac{\sum\limits_{cyc}y_{1}x_{2}x_{3}(x_{2}-x_{3})}{\sum\limits_{cyc}x_{1}x_{2}(x_{1}-x_{2})}\\
\end{aligned}
\]

所以,该二次函数的解析式为
\[y=-\frac{\sum\limits_{cyc}x_{1}(y_{2}-y_{3})}{\sum\limits_{cyc}x_{1}^{2}(y_{2}-y_{3})}x^{2}
+\frac{\sum\limits_{cyc}x_{1}^{2}(y_{2}-y_{3})}{\sum\limits_{cyc}x_{1}^{2}(x_{2}-x_{3})}x
+\frac{\sum\limits_{cyc}y_{1}x_{2}x_{3}(x_{2}-x_{3})}{\sum\limits_{cyc}x_{1}x_{2}(x_{1}-x_{2})}\]


\end{document}